Parikh/Eq_Sys.thy
@@ -1,0 +1,134 @@
+theory Eq_Sys
+  imports
+    "./Lfun"
+    "./Parikh_Img"
+begin
+
+section \<open>systems of equations\<close>
+
+(* We just represent the right hand sides *)
+type_synonym 'a eq_sys = "'a lfun list"
+
+(* sys independent on variables \<le> n *)
+definition indep_leq :: "'a eq_sys \<Rightarrow> nat \<Rightarrow> bool" where
+  "indep_leq sys n \<equiv> \<forall>eq \<in> set sys. \<forall>x \<in> vars eq. x > n"
+
+(* solves equation with \<subseteq> *)
+definition solves_ineq_sys :: "'a eq_sys \<Rightarrow> 'a state \<Rightarrow> bool" where
+  "solves_ineq_sys sys s \<equiv> \<forall>i < length sys. eval (sys ! i) s \<subseteq> s i"
+
+(* solves equation with = *)
+definition solves_eq_sys :: "'a eq_sys \<Rightarrow> 'a state \<Rightarrow> bool" where
+  "solves_eq_sys sys s \<equiv> \<forall>i < length sys. eval (sys ! i) s = s i"
+
+(* solves equation with \<subseteq>, only caring about the Parikh image *)
+definition solves_ineq_comm :: "nat \<Rightarrow> 'a lfun \<Rightarrow> 'a state \<Rightarrow> bool" where
+  "solves_ineq_comm x eq s \<equiv> parikh_img (eval eq s) \<subseteq> parikh_img (s x)"
+
+(* solves equation system with \<subseteq>, only caring about the Parikh image *)
+definition solves_ineq_sys_comm :: "'a eq_sys \<Rightarrow> 'a state \<Rightarrow> bool" where
+  "solves_ineq_sys_comm sys s \<equiv> \<forall>i < length sys. solves_ineq_comm i (sys ! i) s"
+
+(* solves equation with =, only caring about the Parikh image*)
+definition solves_eq_comm :: "nat \<Rightarrow> 'a lfun \<Rightarrow> 'a state \<Rightarrow> bool" where
+  "solves_eq_comm x eq s \<equiv> parikh_img (eval eq s) = parikh_img (s x)"
+
+(* solves equation system with =, only caring about the Parikh image *)
+definition solves_eq_sys_comm :: "'a eq_sys \<Rightarrow> 'a state \<Rightarrow> bool" where
+  "solves_eq_sys_comm sys s \<equiv> \<forall>i < length sys. solves_eq_comm i (sys ! i) s"
+
+(* Substituion into each equation of a system *)
+definition sys_subst :: "'a eq_sys \<Rightarrow> (nat \<Rightarrow> 'a lfun) \<Rightarrow> 'a eq_sys" where
+  "sys_subst sys s \<equiv> map (\<lambda>eq. subst eq s) sys"
+
+definition partial_sol_ineq :: "nat \<Rightarrow> 'a lfun \<Rightarrow> 'a lfun \<Rightarrow> bool" where
+  "partial_sol_ineq x eq sol \<equiv> \<forall>s. s x = eval sol s \<longrightarrow> solves_ineq_comm x eq s"
+
+definition solution_ineq_sys :: "'a eq_sys \<Rightarrow> (nat \<Rightarrow> 'a lfun) \<Rightarrow> bool" where
+  "solution_ineq_sys sys sols \<equiv> \<forall>s. (\<forall>x. s x = eval (sols x) s) \<longrightarrow> solves_ineq_sys_comm sys s"
+
+definition partial_min_sol_ineq_sys :: "nat \<Rightarrow> 'a eq_sys \<Rightarrow> (nat \<Rightarrow> 'a lfun) \<Rightarrow> bool" where
+  "partial_min_sol_ineq_sys n sys sols \<equiv>
+    solution_ineq_sys (take n sys) sols \<and>
+    (\<forall>i \<ge> n. sols i = V i) \<and>
+    (\<forall>i < n. \<forall>x \<in> vars (sols i). x \<ge> n \<and> x < length sys) \<and>
+    (\<forall>sols' s'. (\<forall>x. s' x = eval (sols' x) s')
+                  \<and> solves_ineq_sys_comm (take n sys) s'
+                  \<longrightarrow> (\<forall>i. parikh_img (eval (sols i) s') \<subseteq> parikh_img (s' i)))"
+
+
+definition partial_min_sol_one_ineq :: "nat \<Rightarrow> 'a lfun \<Rightarrow> 'a lfun \<Rightarrow> bool" where
+  "partial_min_sol_one_ineq x eq sol \<equiv>
+    partial_sol_ineq x eq sol \<and>
+    vars sol \<subseteq> vars eq - {x} \<and>
+    (\<forall>sol' s'. solves_ineq_comm x eq s' \<and> s' x = eval sol' s'
+               \<longrightarrow> parikh_img (eval sol s') \<subseteq> parikh_img (s' x))"
+
+definition min_sol_ineq_sys :: "'a eq_sys \<Rightarrow> 'a state \<Rightarrow> bool" where
+  "min_sol_ineq_sys sys sol \<equiv>
+    solves_ineq_sys_comm sys sol \<and>
+    (\<forall>sol'. solves_ineq_sys_comm sys sol' \<longrightarrow> (\<forall>x. parikh_img (sol x) \<subseteq> parikh_img (sol' x)))"
+
+(* TODO: currently unused *)
+definition partial_sol_eq :: "nat \<Rightarrow> 'a lfun \<Rightarrow> 'a lfun \<Rightarrow> bool" where
+  "partial_sol_eq x eq sol \<equiv> \<forall>s. s x = eval sol s \<longrightarrow> solves_eq_comm x eq s"
+
+
+lemma partial_sol_ineqI:
+  assumes "\<And>s. s x = eval sol s \<Longrightarrow> parikh_img (eval (subst eq (V(x := sol))) s) \<subseteq> parikh_img (s x)"
+    shows "partial_sol_ineq x eq sol"
+unfolding partial_sol_ineq_def solves_ineq_comm_def proof (rule allI, rule impI)
+  fix s
+  assume x_is_sol: "s x = eval sol s"
+
+  from x_is_sol have "s = s(x := eval sol s)" using fun_upd_triv by metis
+  then have "eval eq s = eval (subst eq (V(x := sol))) s"
+    using substitution_lemma_update[of eq] by simp
+  with assms x_is_sol show "parikh_img (eval eq s) \<subseteq> parikh_img (s x)" by simp
+qed
+
+
+lemma partial_sol_eqI:
+  assumes "\<And>s. s x = eval sol s \<Longrightarrow> parikh_img (eval (subst eq (V(x := sol))) s) = parikh_img (s x)"
+    shows "partial_sol_eq x eq sol"
+unfolding partial_sol_eq_def solves_eq_comm_def proof (rule allI, rule impI)
+  fix s
+  assume x_is_sol: "s x = eval sol s"
+  
+  from x_is_sol have "s = s(x := eval sol s)" using fun_upd_triv by metis
+  then have "eval eq s = eval (subst eq (V(x := sol))) s"
+    using substitution_lemma_update[of eq] by simp
+  with assms x_is_sol show "parikh_img (eval eq s) = parikh_img (s x)" by simp
+qed
+
+
+lemma sys_subst_subst:
+  assumes "i < length sys"
+  shows "(sys_subst sys s) ! i = subst (sys ! i) s"
+  unfolding sys_subst_def by (simp add: assms)
+
+
+(* TODO: currently unused *)
+lemma sol_Suc_n_sol_n:
+  assumes "solution_ineq_sys (take (Suc n) sys) sols"
+  shows "solution_ineq_sys (take n sys) sols"
+  using assms unfolding solution_ineq_sys_def solves_ineq_sys_comm_def by auto
+
+
+lemma same_min_sol_if_same_parikh_img:
+  assumes same_parikh_img: "\<forall>s. parikh_img (eval f s) = parikh_img (eval g s)"
+      and same_vars:       "vars f - {x} = vars g - {x}"
+      and minimal_sol:     "partial_min_sol_one_ineq x f sol"
+    shows                  "partial_min_sol_one_ineq x g sol"
+proof -
+  from minimal_sol have "vars sol \<subseteq> vars g - {x}"
+    unfolding partial_min_sol_one_ineq_def using same_vars by blast
+  moreover from same_parikh_img minimal_sol have "partial_sol_ineq x g sol"
+    unfolding partial_min_sol_one_ineq_def partial_sol_ineq_def solves_ineq_comm_def by simp
+  moreover from same_parikh_img minimal_sol have "\<forall>sol' s'. solves_ineq_comm x g s' \<and> s' x = eval sol' s'
+               \<longrightarrow> parikh_img (eval sol s') \<subseteq> parikh_img (s' x)"
+    unfolding partial_min_sol_one_ineq_def solves_ineq_comm_def by blast
+  ultimately show ?thesis unfolding partial_min_sol_one_ineq_def by fast
+qed
+
+end
